Start proving that in the absence of early errors, the translation function always yields a valid translation

WarblreEquiv/RegexpTranslation.v
@@ -1,13 +1,14 @@
 From Warblre Require Import Patterns Result Errors Coercions Notation Base StaticSemantics.
 From Warblre Require Characters.
 From Warblre Require EarlyErrors.
-From Linden Require Import Regex LWParameters Parameters Chars Groups.
+From Linden Require Import Regex LWParameters Parameters Chars Groups Tactics.
 Import Notation.
 Import Result.
 Import Result.Notations.
 Local Open Scope result_flow.
 Require Import List.
 Import ListNotations.
+Require Import PeanoNat Lia.
 
 (** * Relation defining equivalence between Warblre regexes and Linden regexes *)
 
@@ -212,22 +213,232 @@ Section RegexpTranslation.
   Definition equiv_regex (wreg: Patterns.Regex) (lreg: regex) := equiv_regex' wreg lreg 0 (buildnm wreg).
 
 
+  Section Lemmas.
+
+    (* Two equivalent regexes have the same number of capturing groups. *)
+    Lemma num_groups_equiv:
+      forall wreg lreg n nm,
+        equiv_regex' wreg lreg n nm ->
+        num_groups lreg = countLeftCapturingParensWithin_impl wreg.
+    Proof.
+      intros wreg lreg n nm Hequiv.
+      induction Hequiv as [
+        n |
+        n c |
+          n |
+          n |
+          n |
+          esc cd n Hequivesc |
+          esc cd n Hequivesc |
+          cc cd n Hequivcc |
+          n wr1 wr2 lr1 lr2 Hequiv1 IH1 Hequiv2 IH2 |
+        n wr1 wr2 lr1 lr2 Hequiv1 IH1 Hequiv2 IH2 |
+        n wr lr wquant lquant wgreedylazy greedy Hequiv IH Hequivquant Hequivgreedy |
+          name n wr lr Hequiv IH |
+          name n wr lr Hequiv IH |
+        n nm wr lr wlk llk Hequiv IH Hequivlk |
+        n nm wr lanchor Hanchequiv]; simpl; try lia; try reflexivity.
+      - inversion Hequivquant; inversion Hequivgreedy; auto.
+      - inversion Hequivlk; auto.
+      - inversion Hanchequiv; auto.
+    Qed.
+  End Lemmas.
+
+  Section Buildnm_GSMatch.
+
+    (** * Linking name maps and StaticSemantics.groupSpecifiersThatMatch *)
+    (* Function mapping a RegexNode to a possible item in a name map *)
+    Definition regexnode_nmitem (r0: Node.RegexNode) :=
+      let (y, ctx0) := r0 in
+      match y with
+      | Patterns.Group (Some gs) inner =>
+        [(gs, StaticSemantics.countLeftCapturingParensBefore y ctx0 + 1)]
+      | _ => []
+      end.
+
+    Lemma buildnm'_spec:
+      forall nm wr ctx n,
+        n = StaticSemantics.countLeftCapturingParensBefore wr ctx ->
+        buildnm' wr nm n =
+          (List.rev (
+            List.flat_map regexnode_nmitem (NodeProps.Zipper.Walk.walk wr ctx)
+          ) ++ nm,
+          n + StaticSemantics.countLeftCapturingParensWithin wr ctx).
+    Proof.
+      intros nm wr. revert nm.
+      induction wr; simpl; try solve[intros; rewrite Nat.add_0_r; reflexivity].
+      - intros nm ctx n Heqn. rewrite IHwr1 with (ctx := Node.Disjunction_left wr2 :: ctx).
+        2: { simpl. unfold StaticSemantics.countLeftCapturingParensBefore in *. lia. }
+        rewrite IHwr2 with (ctx := Node.Disjunction_right wr1 :: ctx).
+        2: { simpl. unfold countLeftCapturingParensWithin, countLeftCapturingParensBefore in *. lia. }
+        f_equal. 2: unfold countLeftCapturingParensWithin; lia.
+        rewrite flat_map_app, rev_app_distr, app_assoc. reflexivity.
+      - intros nm ctx n Heqn. apply IHwr with (ctx := Node.Quantified_inner q :: ctx).
+        simpl. unfold countLeftCapturingParensBefore in *. lia.
+      - intros nm ctx n Heqn. rewrite IHwr1 with (ctx := Node.Seq_left wr2 :: ctx).
+        2: { simpl. unfold StaticSemantics.countLeftCapturingParensBefore in *. lia. }
+        rewrite IHwr2 with (ctx := Node.Seq_right wr1 :: ctx).
+        2: { simpl. unfold countLeftCapturingParensWithin, countLeftCapturingParensBefore in *. lia. }
+        f_equal. 2: unfold countLeftCapturingParensWithin; lia.
+        rewrite flat_map_app, rev_app_distr, app_assoc. reflexivity.
+      - (* Group: interesting case *)
+        intros nm ctx n Heqn. destruct name as [name|].
+        + rewrite IHwr with (ctx := Node.Group_inner (Some name) :: ctx).
+          2: { simpl. unfold countLeftCapturingParensBefore in *. lia. }
+          f_equal.
+          2: { unfold countLeftCapturingParensWithin. lia. }
+          rewrite rev_app_distr. simpl. rewrite <- app_assoc. simpl. f_equal.
+          f_equal. f_equal. setoid_rewrite <- Heqn. lia.
+        + rewrite IHwr with (ctx := Node.Group_inner None :: ctx).
+          2: { simpl. unfold countLeftCapturingParensBefore in *. lia. }
+          f_equal. unfold countLeftCapturingParensWithin in *. lia.
+      - intros nm ctx n Heqn. apply IHwr with (ctx := Node.Lookahead_inner :: ctx).
+        simpl. unfold countLeftCapturingParensBefore in *. lia.
+      - intros nm ctx n Heqn. apply IHwr with (ctx := Node.NegativeLookahead_inner :: ctx).
+        simpl. unfold countLeftCapturingParensBefore in *. lia.
+      - intros nm ctx n Heqn. apply IHwr with (ctx := Node.Lookbehind_inner :: ctx).
+        simpl. unfold countLeftCapturingParensBefore in *. lia.
+      - intros nm ctx n Heqn. apply IHwr with (ctx := Node.NegativeLookbehind_inner :: ctx).
+        simpl. unfold countLeftCapturingParensBefore in *. lia.
+    Qed.
+
+    Lemma buildnm_spec:
+      forall wr,
+        buildnm wr = List.rev (List.flat_map regexnode_nmitem (NodeProps.Zipper.Walk.walk wr nil)).
+    Proof.
+      intro wr. unfold buildnm.
+      rewrite buildnm'_spec with (ctx := []) by reflexivity.
+      rewrite app_nil_r. reflexivity.
+    Qed.
+
+    Lemma buildnm_gsmatch:
+      forall l nm r ctx name,
+        l = StaticSemantics.groupSpecifiersThatMatch r ctx name ->
+        nm = buildnm (Node.zip r ctx) ->
+        forall gid,
+          In (name, gid) nm <->
+          In gid (List.map (fun '(fst, snd) => StaticSemantics.countLeftCapturingParensBefore fst snd) l).
+    Proof.
+      intros l nm r ctx name -> -> gid.
+      rewrite buildnm_spec.
+      rewrite <- In_rev.
+      rewrite in_flat_map.
+      unfold groupSpecifiersThatMatch.
+      rewrite in_map_iff. setoid_rewrite in_flat_map.
+      split.
+      - intros [[regsub ctxsub] [CHILD NMITEM]]. unfold regexnode_nmitem in NMITEM.
+        destruct regsub; try solve[inversion NMITEM].
+        destruct name0; try solve[inversion NMITEM].
+        destruct NMITEM as [NMITEM | NMITEM]; try solve[inversion NMITEM].
+        injection NMITEM as -> Heqgid.
+        exists (regsub, Node.Group_inner (Some name) :: ctxsub).
+        split. 1: { simpl. unfold countLeftCapturingParensBefore in *. lia. }
+        eexists. split. 1: apply CHILD.
+        simpl.
+        destruct (string_eq_dec _ _). 2: contradiction.
+        left. reflexivity.
+      - intros [[reg_inner ctx_inner] [Heqgid [[regsub ctxsub] [CHILD GS]]]].
+        destruct regsub; try solve[inversion GS].
+        destruct name0; try solve[inversion GS].
+        destruct (g ==# capturingGroupName name)%wt; try solve[inversion GS].
+        unfold capturingGroupName in e. subst g.
+        eexists. split. 1: apply CHILD.
+        destruct GS as [GS|GS]; try solve[inversion GS].
+        injection GS as <- <-. simpl.
+        left. f_equal. simpl in Heqgid. unfold countLeftCapturingParensBefore in *. lia.
+    Qed.
+
+    Lemma unique_In_eq {A F} `{Ferr: Result.AssertionError F}:
+      forall l: list A, length l = 1 ->
+        forall x, List.List.Unique.unique l = Success x <-> In x l.
+    Proof.
+      intros l Hlen x. split; intro H.
+      - rewrite List.List.Unique.success with (v := x) by auto. left. reflexivity.
+      - destruct l as [|y l]; try discriminate. destruct l; try discriminate.
+        simpl. destruct H. 2: inversion H.
+        f_equal. auto.
+    Qed.
+
+    Lemma findA_filter {A B}:
+      forall (f: A -> bool) (l: list (A * B)),
+        SetoidList.findA f l =
+        match List.filter (fun '(a, b) => f a) l with
+        | [] => None
+        | (a, b)::_ => Some b
+        end.
+    Proof.
+      induction l; simpl; auto.
+      destruct a as [a b].
+      destruct (f0 a); auto.
+    Qed.
+
+    Lemma in_len1_eq {A}:
+      forall (x y: A) (l: list A),
+        length l = 1 -> In x l -> In y l -> x = y.
+    Proof.
+      intros x y [|a []]; try discriminate.
+      intros _ Hxin Hyin.
+      destruct Hxin as [ <- | [] ].
+      destruct Hyin as [ <- | [] ].
+      reflexivity.
+    Qed.
+
+    Lemma buildnm_gsmatch_unique {F} `{Ferr: Result.AssertionError F}:
+      forall l nm r ctx name gs,
+        l = StaticSemantics.groupSpecifiersThatMatch r ctx name ->
+        length l = 1 ->
+        nm = buildnm (Node.zip r ctx) ->
+        List.List.Unique.unique l = Success gs ->
+        nameidx nm name = Some (StaticSemantics.countLeftCapturingParensBefore (fst gs) (snd gs)).
+    Proof.
+      intros l nm r ctx name gs -> Hlen -> Heqgs.
+      unfold nameidx.
+      rewrite findA_filter.
+      rewrite unique_In_eq in Heqgs by auto.
+      apply in_map with (f := fun '(fst, snd) => countLeftCapturingParensBefore fst snd) in Heqgs.
+      destruct gs as [reg_inner ctx_inner]; simpl in *.
+      rewrite <- buildnm_gsmatch in Heqgs. 2: reflexivity. 2: reflexivity.
+      destruct filter eqn:Hfilter.
+      1: {
+        exfalso. assert (In (name, countLeftCapturingParensBefore reg_inner ctx_inner) []). {
+          setoid_rewrite <- Hfilter. apply filter_In. split; auto. unfold patname_eqb.
+          destruct patname_eq_dec; auto.
+        }
+        inversion H.
+      }
+      assert (In p (filter (fun '(a, _) => patname_eqb a name) (buildnm (Node.zip r ctx)))). {
+        rewrite Hfilter. left. reflexivity.
+      }
+      rewrite filter_In in H. destruct p as [name0 gid].
+      destruct H as [Hin H].
+      unfold patname_eqb in H.
+      destruct patname_eq_dec; try discriminate. subst name0.
+      rewrite buildnm_gsmatch in Hin. 3: reflexivity. 2: reflexivity.
+      rewrite buildnm_gsmatch in Heqgs. 3: reflexivity. 2: reflexivity.
+      f_equal.
+      remember ((map (fun '(fst, snd) => countLeftCapturingParensBefore fst snd)
+            (groupSpecifiersThatMatch _ ctx name))) as l0 in *.
+      apply in_len1_eq with (l := l0); auto.
+      rewrite Heql0, map_length. auto.
+    Qed.
+  End Buildnm_GSMatch.
+
   (* Translation function from Warblre to Linden. *)
   Section WarblreToLinden.
 
     Inductive wl_transl_error: Type :=
       | WlMalformed.
 
-    Definition characterClassEsc_to_linden (esc: Patterns.CharacterClassEscape): Result char_descr wl_transl_error :=
+    Definition characterClassEsc_to_linden (esc: Patterns.CharacterClassEscape): char_descr :=
       match esc with
-      | Patterns.esc_d => Success CdDigits
-      | Patterns.esc_D => Success CdNonDigits
-      | Patterns.esc_s => Success CdWhitespace
-      | Patterns.esc_S => Success CdNonWhitespace
-      | Patterns.esc_w => Success CdWordChar
-      | Patterns.esc_W => Success CdNonWordChar
-      | Patterns.UnicodeProp p => Success (CdUnicodeProp p)
-      | Patterns.UnicodePropNeg p => Success (CdNonUnicodeProp p)
+      | Patterns.esc_d => CdDigits
+      | Patterns.esc_D => CdNonDigits
+      | Patterns.esc_s => CdWhitespace
+      | Patterns.esc_S => CdNonWhitespace
+      | Patterns.esc_w => CdWordChar
+      | Patterns.esc_W => CdNonWordChar
+      | Patterns.UnicodeProp p => CdUnicodeProp p
+      | Patterns.UnicodePropNeg p => CdNonUnicodeProp p
       end.
 
     Definition controlEsc_singleCharacter (esc: Patterns.ControlEscape): Parameters.Character :=
@@ -243,27 +454,27 @@ Section RegexpTranslation.
       let n := NonNegInt.modulo (AsciiLetter.numeric_value l) 32 in
       Character.from_numeric_value n.
     
-    Definition characterEscape_singleCharacter (esc: Patterns.CharacterEscape): Result Parameters.Character wl_transl_error :=
+    Definition characterEscape_singleCharacter (esc: Patterns.CharacterEscape): Parameters.Character :=
       match esc with
-      | Patterns.ControlEsc esc => Success (controlEsc_singleCharacter esc)
-      | Patterns.AsciiControlEsc l => Success (asciiEsc_singleCharacter l)
-      | Patterns.esc_Zero => Success (Character.from_numeric_value 0)
-      | Patterns.HexEscape d1 d2 => Success (Character.from_numeric_value (HexDigit.to_integer_2 d1 d2))
-      | Patterns.UnicodeEsc (Patterns.Pair head tail) => Success (Character.from_numeric_value (unicodeCodePoint head tail))
-      | Patterns.UnicodeEsc (Patterns.Lonely hex) => Success (Character.from_numeric_value (StaticSemantics.characterValue_Hex4Digits hex))
-      | Patterns.UnicodeEsc (Patterns.CodePoint c) => Success c
-      | Patterns.IdentityEsc c => Success c
+      | Patterns.ControlEsc esc => controlEsc_singleCharacter esc
+      | Patterns.AsciiControlEsc l => asciiEsc_singleCharacter l
+      | Patterns.esc_Zero => Character.from_numeric_value 0
+      | Patterns.HexEscape d1 d2 => Character.from_numeric_value (HexDigit.to_integer_2 d1 d2)
+      | Patterns.UnicodeEsc (Patterns.Pair head tail) => Character.from_numeric_value (unicodeCodePoint head tail)
+      | Patterns.UnicodeEsc (Patterns.Lonely hex) => Character.from_numeric_value (StaticSemantics.characterValue_Hex4Digits hex)
+      | Patterns.UnicodeEsc (Patterns.CodePoint c) => c
+      | Patterns.IdentityEsc c => c
       end.
 
     Definition characterEscape_to_linden (esc: Patterns.CharacterEscape): Result char_descr wl_transl_error :=
-      let! c =<< characterEscape_singleCharacter esc in
+      let c := characterEscape_singleCharacter esc in
       Success (CdSingle c).
 
     Definition atomesc_to_linden (ae: Patterns.AtomEscape) (nm:namedmap): Result regex wl_transl_error :=
       match ae with
       | Patterns.DecimalEsc gid => Success (Backreference (positive_to_nat gid))
       | Patterns.ACharacterClassEsc esc => 
-          let! cd =<< characterClassEsc_to_linden esc in
+          let cd := characterClassEsc_to_linden esc in
           Success (Character cd)
       | Patterns.ACharacterEsc esc => 
           let! cd =<< characterEscape_to_linden esc in
@@ -279,7 +490,7 @@ Section RegexpTranslation.
       match esc with
       | Patterns.esc_b => Success (CdSingle Characters.BACKSPACE)
       | Patterns.esc_Dash => Success (CdSingle Characters.HYPHEN_MINUS)
-      | Patterns.CCharacterClassEsc esc => characterClassEsc_to_linden esc
+      | Patterns.CCharacterClassEsc esc => Success (characterClassEsc_to_linden esc)
       | Patterns.CCharacterEsc esc => characterEscape_to_linden esc
       end.
 
@@ -288,7 +499,7 @@ Section RegexpTranslation.
       | Patterns.esc_b => Success Characters.BACKSPACE
       | Patterns.esc_Dash => Success Characters.HYPHEN_MINUS
       | Patterns.CCharacterClassEsc esc => Error WlMalformed
-      | Patterns.CCharacterEsc esc => characterEscape_singleCharacter esc
+      | Patterns.CCharacterEsc esc => Success (characterEscape_singleCharacter esc)
       end.
     
     Definition classAtom_to_linden (ca: Patterns.ClassAtom): Result char_descr wl_transl_error :=
@@ -496,11 +707,11 @@ Section RegexpTranslation.
 
     Lemma characterClassEsc_to_linden_sound:
       forall esc cd,
-        characterClassEsc_to_linden esc = Success cd ->
+        characterClassEsc_to_linden esc = cd ->
         equiv_CharacterClassEscape esc cd.
     Proof.
       intro esc. destruct esc; simpl; try discriminate.
-      all: intros cd H; injection H as <-; constructor.
+      all: intros cd <-; constructor.
     Qed.
 
     Lemma controlEsc_singleCharacter_sound:
@@ -535,11 +746,8 @@ Section RegexpTranslation.
       intro ae. destruct ae.
       - simpl. intros lr gid nm H. injection H as <-. constructor.
       - simpl. intros lr n nm.
-        destruct characterClassEsc_to_linden as [cd|] eqn:Hcd; try discriminate. simpl.
         intro H. injection H as <-. constructor. apply characterClassEsc_to_linden_sound. auto.
-      - simpl. intros lr n nm.
-        destruct characterEscape_to_linden as [cd|] eqn:Hcd; try discriminate. simpl.
-        intro H. injection H as <-. constructor. apply characterEscape_to_linden_sound. auto.
+      - simpl. intros lr n nm H. injection H as <-. constructor. apply characterEscape_to_linden_sound. auto.
       - simpl. intros lr n nm H. destruct (nameidx nm id) eqn:NAME; [|discriminate].
         inversion H. subst. constructor. auto.
     Qed.
@@ -563,7 +771,7 @@ Section RegexpTranslation.
       intros esc cda. destruct esc; simpl.
       - intro H. injection H as <-. constructor.
       - intro H. injection H as <-. constructor.
-      - intro H. constructor. apply characterClassEsc_to_linden_sound. auto.
+      - intro H. injection H as <-. constructor. apply characterClassEsc_to_linden_sound. auto.
       - intro H. constructor. apply characterEscape_to_linden_sound. auto.
     Qed.
 
@@ -579,12 +787,12 @@ Section RegexpTranslation.
 
     Lemma characterEscape_singleCharacter_sound:
       forall esc clh,
-        characterEscape_singleCharacter esc = Success clh ->
+        characterEscape_singleCharacter esc = clh ->
         equiv_CharacterEscape esc (CdSingle clh).
     Proof.
       intros esc clh. destruct esc; simpl; try discriminate.
       5: destruct seq; simpl.
-      all: intro H; injection H as <-; constructor.
+      all: intros <-; constructor.
       - apply controlEsc_singleCharacter_sound.
       - apply asciiEsc_singleCharacter_sound.
     Qed.
@@ -597,7 +805,7 @@ Section RegexpTranslation.
       intros esc clh. destruct esc; simpl; try discriminate.
       - intro H. injection H as <-. constructor.
       - intro H. injection H as <-. constructor.
-      - intro H. constructor. apply characterEscape_singleCharacter_sound. auto.
+      - intro H. injection H as <-. constructor. apply characterEscape_singleCharacter_sound. auto.
     Qed.
 
     Lemma classAtom_singleCharacter_sound:
@@ -704,6 +912,171 @@ Section RegexpTranslation.
     Qed.
 
   End TranslationSoundness.
+
+  Section TranslationCompleteness.
+
+    Lemma EarlyErrors_Down:
+      forall wrout ctxout wrin ctxin,
+        NodeProps.Zipper.Down (wrin, ctxin) (wrout, ctxout) ->
+        EarlyErrors.Pass_Regex wrout ctxout ->
+        EarlyErrors.Pass_Regex wrin ctxin.
+    Proof.
+      intros wrout ctxout wrin ctxin DOWN EE.
+      inversion DOWN; subst; inversion EE; subst; auto.
+    Qed.
+
+    Lemma EarlyErrors_Downstar:
+      forall x y,
+        NodeProps.Zipper.Down_Star x y ->
+        EarlyErrors.Pass_Regex (fst y) (snd y) ->
+        EarlyErrors.Pass_Regex (fst x) (snd x).
+    Proof.
+      intros x y DOWN_STAR EE.
+      induction DOWN_STAR.
+      - destruct x as [wrin ctxin]. destruct y as [wrout ctxout]. eauto using EarlyErrors_Down.
+      - auto.
+      - auto.
+    Qed.
+
+    Lemma EarlyErrors_sub:
+      forall wroot,
+        EarlyErrors.Pass_Regex wroot nil ->
+        forall wr ctx,
+          Node.Root wroot (wr, ctx) ->
+          EarlyErrors.Pass_Regex wr ctx.
+    Proof.
+      intros wroot EE wr ctx ROOT.
+      apply NodeProps.Zipper.Down.root_is_top in ROOT.
+      apply EarlyErrors_Downstar with (x := (wr, ctx)) (y := (wroot, [])); auto.
+    Qed.
+
+    Theorem earlyErrors_pass_translation':
+      forall wroot: Patterns.Regex,
+        (*EarlyErrors.Pass_Regex wroot nil ->*) (* This does not include the condition on the absence of duplicate groups *)
+        earlyErrors wroot nil = Success false -> (* This does, and Warblre already proves that earlyErrors can never fail (section Safety in Warblre.props.EarlyErrors) *)
+        forall wr ctx,
+          Node.Root wroot (wr, ctx) ->
+          exists lr, warblre_to_linden wr (StaticSemantics.countLeftCapturingParensBefore wr ctx) (buildnm wroot) = Success lr.
+    Proof.
+      intros wroot EE0. pose proof EarlyErrors.earlyErrors wroot EE0 as H.
+      induction wr; simpl.
+      - intros ctx _. eexists. reflexivity.
+      - intros ctx _. eexists. reflexivity.
+      - intros ctx _. eexists. reflexivity.
+      - intros ctx Hroot.
+        pose proof EarlyErrors_sub wroot H _ ctx Hroot as EE.
+        inversion EE; subst. inversion H1; subst.
+        + simpl. eexists. reflexivity.
+        + simpl. eexists. reflexivity.
+        + simpl. eexists. reflexivity.
+        + simpl.
+          destruct groupSpecifiersThatMatch as [|gs []] eqn:Heqgs; try discriminate.
+          rewrite <- Heqgs in H0. erewrite buildnm_gsmatch_unique.
+          3: apply H0.
+          2: reflexivity.
+          2: rewrite Hroot; reflexivity.
+          2: rewrite Heqgs; reflexivity.
+          eexists. reflexivity.
+      - intros ctx Hroot.
+        pose proof EarlyErrors_sub wroot H _ ctx Hroot as EE.
+        inversion EE; subst. inversion H1; subst.
+        + simpl. admit.
+        + simpl. admit.
+      - intros ctx Hroot.
+        specialize (IHwr1 (Node.Disjunction_left wr2 :: ctx)).
+        specialize_prove IHwr1 by eauto using NodeProps.Zipper.Down.same_root_down0, NodeProps.Zipper.Down_Disjunction_left.
+        destruct IHwr1 as [lr1 IHwr1].
+        specialize (IHwr2 (Node.Disjunction_right wr1 :: ctx)).
+        specialize_prove IHwr2 by eauto using NodeProps.Zipper.Down.same_root_down0, NodeProps.Zipper.Down_Disjunction_right.
+        destruct IHwr2 as [lr2 IHwr2].
+        simpl in *. rewrite Nat.add_0_r in IHwr1. setoid_rewrite IHwr1. simpl.
+        rewrite num_groups_equiv with (wreg := wr1) (n := @countLeftCapturingParensBefore (@LWParameters params) wr1 ctx) (nm := buildnm wroot).
+        2: { apply warblre_to_linden_sound. auto. }
+        rewrite Nat.add_comm. setoid_rewrite IHwr2. simpl. eexists. reflexivity.
+      - intros ctx Hroot.
+        pose proof EarlyErrors_sub wroot H _ ctx Hroot as EE.
+        specialize (IHwr (Node.Quantified_inner q :: ctx)).
+        specialize_prove IHwr by eauto using NodeProps.Zipper.Down.same_root_down0, NodeProps.Zipper.Down_Quantified_inner.
+        destruct IHwr as [lrsub IHwr].
+        inversion EE; subst. inversion H4; subst.
+        + inversion H0; subst.
+          * simpl. simpl in IHwr. rewrite Nat.add_0_r in IHwr. setoid_rewrite IHwr. simpl. eexists. reflexivity.
+          * simpl. simpl in IHwr. rewrite Nat.add_0_r in IHwr. setoid_rewrite IHwr. simpl. eexists. reflexivity.
+          * simpl. simpl in IHwr. rewrite Nat.add_0_r in IHwr. setoid_rewrite IHwr. simpl. eexists. reflexivity.
+          * simpl. simpl in IHwr. rewrite Nat.add_0_r in IHwr. setoid_rewrite IHwr. simpl. eexists. reflexivity.
+          * simpl. simpl in IHwr. rewrite Nat.add_0_r in IHwr. setoid_rewrite IHwr. simpl. eexists. reflexivity.
+          * simpl. apply Nat.leb_le in H1. rewrite H1. simpl. simpl in IHwr. rewrite Nat.add_0_r in IHwr. setoid_rewrite IHwr. simpl. eexists. reflexivity.
+        + inversion H0; subst.
+          * simpl. simpl in IHwr. rewrite Nat.add_0_r in IHwr. setoid_rewrite IHwr. simpl. eexists. reflexivity.
+          * simpl. simpl in IHwr. rewrite Nat.add_0_r in IHwr. setoid_rewrite IHwr. simpl. eexists. reflexivity.
+          * simpl. simpl in IHwr. rewrite Nat.add_0_r in IHwr. setoid_rewrite IHwr. simpl. eexists. reflexivity.
+          * simpl. simpl in IHwr. rewrite Nat.add_0_r in IHwr. setoid_rewrite IHwr. simpl. eexists. reflexivity.
+          * simpl. simpl in IHwr. rewrite Nat.add_0_r in IHwr. setoid_rewrite IHwr. simpl. eexists. reflexivity.
+          * simpl. apply Nat.leb_le in H1. rewrite H1. simpl. simpl in IHwr. rewrite Nat.add_0_r in IHwr. setoid_rewrite IHwr. simpl. eexists. reflexivity.
+      - (* Sequence: similar to disjunction *)
+        intros ctx Hroot.
+        specialize (IHwr1 (Node.Seq_left wr2 :: ctx)).
+        specialize_prove IHwr1 by eauto using NodeProps.Zipper.Down.same_root_down0.
+        destruct IHwr1 as [lr1 IHwr1].
+        specialize (IHwr2 (Node.Seq_right wr1 :: ctx)).
+        specialize_prove IHwr2 by eauto using NodeProps.Zipper.Down.same_root_down0.
+        destruct IHwr2 as [lr2 IHwr2].
+        simpl in *. rewrite Nat.add_0_r in IHwr1. setoid_rewrite IHwr1. simpl.
+        rewrite num_groups_equiv with (wreg := wr1) (n := @countLeftCapturingParensBefore (@LWParameters params) wr1 ctx) (nm := buildnm wroot).
+        2: { apply warblre_to_linden_sound. auto. }
+        rewrite Nat.add_comm. setoid_rewrite IHwr2. simpl. eexists. reflexivity.
+      - (* Group *)
+        intros ctx Hroot.
+        specialize (IHwr (Node.Group_inner name :: ctx)).
+        specialize_prove IHwr by eauto using NodeProps.Zipper.Down.same_root_down0.
+        destruct IHwr as [lrsub IHwr].
+        simpl in IHwr. rewrite Nat.add_comm in IHwr.
+        pose proof EarlyErrors_sub wroot H _ ctx Hroot as EE.
+        destruct name as [name|].
+        + unfold earlyErrors in EE0.
+          destruct List.List.Exists.exist eqn:Hdup; try discriminate.
+          destruct s; try discriminate.
+          apply EarlyErrors.groupSpecifiersThatMatch_singleton with (name := name) in Hdup.
+          assert (Hpres: In (wr, Node.Group_inner (Some name) :: ctx) (groupSpecifiersThatMatch wroot [] name)). {
+            admit. (* Follows from Hroot; non-trivial *)
+          }
+          remember (groupSpecifiersThatMatch wroot [] name) as l in *.
+          destruct l as [|gs []].
+          1: inversion Hpres. 2: { simpl in Hdup. lia. }
+          rewrite buildnm_gsmatch_unique with (l := [gs]) (r := wroot) (ctx := nil) (gs := gs); auto.
+          destruct Hpres as [Hpres | Hpres]; try solve[inversion Hpres].
+          subst gs. simpl.
+          unfold assert_idx_eq. rewrite Nat.add_comm. rewrite Nat.eqb_refl. simpl.
+          setoid_rewrite IHwr. eexists. reflexivity.
+        + setoid_rewrite IHwr. eexists. reflexivity.
+      - intros ctx _. eexists. reflexivity.
+      - intros ctx _. eexists. reflexivity.
+      - intros ctx _. eexists. reflexivity.
+      - intros ctx _. eexists. reflexivity.
+      (* Lookarounds *)
+      - intros ctx Hroot.
+        specialize (IHwr (Node.Lookahead_inner :: ctx)).
+        specialize_prove IHwr by eauto using NodeProps.Zipper.Down.same_root_down0, NodeProps.Zipper.Down_Lookahead_inner.
+        destruct IHwr as [lrsub IHwr]. simpl in *.
+        rewrite Nat.add_0_r in IHwr. setoid_rewrite IHwr. eexists. reflexivity.
+      - intros ctx Hroot.
+        specialize (IHwr (Node.NegativeLookahead_inner :: ctx)).
+        specialize_prove IHwr by eauto using NodeProps.Zipper.Down.same_root_down0, NodeProps.Zipper.Down_NegativeLookahead_inner.
+        destruct IHwr as [lrsub IHwr]. simpl in *.
+        rewrite Nat.add_0_r in IHwr. setoid_rewrite IHwr. eexists. reflexivity.
+      - intros ctx Hroot.
+        specialize (IHwr (Node.Lookbehind_inner :: ctx)).
+        specialize_prove IHwr by eauto using NodeProps.Zipper.Down.same_root_down0, NodeProps.Zipper.Down_Lookbehind_inner.
+        destruct IHwr as [lrsub IHwr]. simpl in *.
+        rewrite Nat.add_0_r in IHwr. setoid_rewrite IHwr. eexists. reflexivity.
+      - intros ctx Hroot.
+        specialize (IHwr (Node.NegativeLookbehind_inner :: ctx)).
+        specialize_prove IHwr by eauto using NodeProps.Zipper.Down.same_root_down0, NodeProps.Zipper.Down_NegativeLookbehind_inner.
+        destruct IHwr as [lrsub IHwr]. simpl in *.
+        rewrite Nat.add_0_r in IHwr. setoid_rewrite IHwr. eexists. reflexivity.
+    Admitted.
+    
+  End TranslationCompleteness.
 
 End RegexpTranslation.
 
